\subsection{Continuous time, finite horizon DP (HJB theory)}
HJB: Hamilton-Jacobi-Bellman%
%
\subsubsection{Problem formulation}
\begin{optExample}{Problem setup}
\begin{align}
\min_{u(.)} & \intdt{t_0}{t_f}{ f_0 \paren{\txu} } + \phi \paren{t_f, x_f} 
\end{align}
\begin{alignat*}{6}
\st{} \quad&&
  \dot{x} &= f \paren{\txu} &&t \in [t_0, t_f]     \\
&& u(t)    &\in \setU{t, x(t)} \subset \R^q\\
&&~ u &\txt{ piecewise continuous}
\end{alignat*}
\end{optExample}

\begin{itemize}
\item Optimal cost to go
    \begin{align}
    J^* \paren{t_1, x_1} = \min_{u(.)}
        \intdt{t_1}{t_f}{ f_0 \paren{\txu} } + \phi \paren{x_f}
    \end{align}
\item Value function
    \begin{align*}
    J \paren{t_0,x)} &= V(x)\\
    \\
    J \paren{t_0,x_0} 
        &\overtext{Def.}{=}
        \min \intdt{t_0}{t_f}{ f_0 \paren{\txu} } + \phi \paren{x_f}\\
        &= \intdt{t_0}{t_f}{ f_0 \paren{\txuOpt} } + \phi \paren{x_f^*}\\
        \begin{split}
            &= \intdt{t_0}{t_1}{ f_0 \paren{\txuOpt} } \\
        &\quad + \underbrace{ \intdt{t_1}{t_f}{ f_0 \paren{\txuOpt} } }_{\txt{PoO } J \paren{t_1,x_1} }
        \end{split}\\
        &= \intdt{t_0}{t_1}{ f_0 \paren{\txuOpt} } + J \paren{t_1,x_1}\\
    \intertext{PoO as a formula:}
    J \paren{t_0,x_0}
        &= \min_{u} \set{ \underbrace{\intdt{t_0}{t_1}{ f_0 \paren{\txu} }}_{\txt{note\footnotemark}} + J \paren{t_1,x_1} }
    \end{align*}
    \footnotetext{'DP recursion' but not as useful as in discrete-time
    since $\intdt{t_0}{t_1}{\dots}$}
\end{itemize}

\subsubsection{Principle of optimality}
\paragraph{Idea} Infinitesimal version of the PoO:
\def\valti{t_0 + \Delta t}
\begin{gather*}
    \begin{align*}
        t_1 = \valti, \quad \Delta t \rightarrow 0,
        ( J \in C^1 )
    \end{align*} \\
    ~\\
    \begin{alignat*}{2}
    & J \paren{t_0,x_0}\\
    =& \min_{u(.)} \set{
        \intdt{t_0}{\valti}{f_0 \paren{\txu}}
        + \underbrace{
            J \paren{\valti, x \paren{\valti}}
            }_{%
            g \paren{\valti{}}, \txt{ note}\footnotemark
            }
        }\\
    =& \min_{u(.)} \left\lbrace
        f_0 \paren{\txuo}\Delta t
        + J \paren{\txuo} \right.\\
        &+  \squareb{
                \pdein{J \paren{\txuo}}{t}
                + \pdein{J \paren{\txuo}}{x}f \paren{\txuo}
                }
            \Delta t\\
        &+ \left.\err(\Delta t^2)
        \right\rbrace\\
    \end{alignat*}
\end{gather*}%
    %
Divide by $\Delta t$:
    \begin{alignat*}{2}
    \cancel{J \paren{t_0,x_0}}
        &=& \min_{u(.)} &\left\lbrace
        f_0 \paren{\txuo} + \cancel{J \paren{\txuo}} \right.\\
        &&&+ \pdein{J \paren{\txuo}}{t} \\
        &&&+ \pdein{J \paren{\txuo}}{x}f \paren{\txuo}\\
        &&&+ \left. \err(\Delta t) \right\rbrace\\
    0
        &=& \min_{u(.)} & \left\lbrace
        f_0 \paren{\txuo} + \pdein{J \paren{\txuo}}{t} \right.\\
        &&& + \pdein{J \paren{\txuo}}{x}f \paren{\txuo} \\
        &&& + \left. \err(\Delta t) \right\rbrace\\
    \end{alignat*}%
$\Delta t \rightarrow 0$:
\begin{alignat*}{3}
& - \pdein{J \paren{t_0,x_0}}{t}\\
    =& \min_{u(.)}  \set{
    f_0 \paren{\txuo}
    + \pdein{J \paren{\txuo}}{x}f \paren{\txuo}
    }      
    \numberthis
    \label{eq:hjb}
    \end{alignat*}
    \footnotetext{$g \paren{\valti} = g(t_0) + \dot{g}(t_0)\Delta t + \err(\Delta t^2)$}%
%
\subsubsection{Hamilton-Jacobi-Bellman equation}
PDE, nonlinear\footnote{nonlinear due to $\min \dots$}
\begin{gather}
\begin{align}
&- \pdein{J \paren{t_0,x_0}}{t} \nonumber \\
    = &\min_{u(.)}  \set{
    f_0 \paren{\txuo}
    + \pdein{J \paren{\txuo}}{x}f \paren{\txuo}
    }
\tag{\ref{eq:hjb}} 
\end{align}\\
    J \paren{t_f,x} = \phi \paren{t_f,x}
    \label{eq:hjb-final}
\end{gather}
    
\begin{figure}[H]
Integration backwards in time.
    \centering
    \def\svgwidth{\columnwidth}
    \footnotesize
    \input{./img/integration-backwards.pdf_tex}
    \label{fig:integration-backwards}
\end{figure}

\subsubsection{Verification theorem}
\begin{theorem}{necessity}
If $J \in C^1$, then $J$ is a solution
of the HJB equation \eqn{eq:hjb}.
\end{theorem}

\begin{theorem}{{sufficiency, verification theorem}}
Suppose $\Jbar{t,x} \in C^1$, and 
    \begin{align}
    - \pdein{\Jbar{t,x}}{t} &= \minux{} \left\lbrace f_0 \paren{\txu} \right. \nonumber \\
    &\quad \left. + \pdein{\Jbar{\txu}}{x} f \paren{\txu} \right\rbrace \tag{\ref{eq:hjb}} \\
    J \paren{t_f,x} &= \phi \paren{t_f,x}
    \tag{\ref{eq:hjb-final}}\\
    \ubar{t,x} &= \argmin \left\lbrace
        f_0 \paren{\txu} \right. \nonumber\\
        & \quad \left. + \pdein{\Jbar{\txu}}{x}f \paren{\txu} \right\rbrace
    \end{align}
Then $\Jbar{} = J$ and $\ubar{}$ is the (an) optimal feedback.
\end{theorem}

\paragraph{Proof:}
\begin{align*}
    g(t_1) - g(t_0) = \intdt{t_0}{t_1}{\dot{g}(t)}
\end{align*}
Find theorem of calculus.\\

\paragraph{Step 1} $\Jbar{} \geq J$
\begin{align*}
- \pdein{\Jbar{t,x}}{t}
        &= \minux{} \left\lbrace f_0 \paren{\txu} \right. \\
        &\quad \left. + \pdein{\Jbar{\txu}}{x}f \paren{\txu} \right\rbrace \\
        &= f_0 \paren{\txuBar} \\
        &\quad + \pdein{\Jbar{\txuBar}}{x}f \paren{\txuBar} \\
-\dot{\Jbar{}}(t,x)
        &= f_0 \paren{\txuBar}\\
\end{align*}
Integrate from $t_0$ to $t_f$:
\begin{align*}
\Jbar{t_0,x_0}
        &= \intdt{t_0}{t_f}{f_0 \paren{\txuBar}} + \Jbar{t_f,x_f}\\
%\Jbar{t_0,x_0}
        &= \intdt{t_0}{t_f}{f_0 \paren{\txuBar}} + \phi \paren{t_f,x_f}
\end{align*}
$\therefore \Jbar{}$ indeed represents the cost to go.

\paragraph{Step 2} $\Jbar{} \leq J, \forall~u(t,x) \in \setU{t,x}$
\begin{align*}
    - \pdein{\Jbar{t,x}}{t}
        &\leq f_0 \paren{\txu} + \pdein{\Jbar{\txu}}{x} f \paren{\txu} \\
-\dot{\Jbar{}}(t,x)
        &\leq f_0 \paren{\txu}
\end{align*}%
%
Integrate from $t_0$ to $t_f$:
\begin{align*}
\Jbar{t_0,x_0}
        &\leq \intdt{t_0}{t_f}{f_0 \paren{\txu}} + \Jbar{t_f,x_f}\\
\Jbar{t_0,x_0}
        &\leq \intdt{t_0}{t_f}{f_0 \paren{\txu}} + \phi \paren{t_f,x_f}\\
        &\qquad \forall~u(t,x) \in \setU{t,x}, \txt{note\footnotemark}\\
\Jbar{t_0,x_0}
        &\leq J \paren{t_0,x_0}
\end{align*}
\footnotetext{Holds also for the optimal feedback $u^*$}

$\ubar{}$ is optimal, because $(\leq) \rightarrow (=)$.

\paragraph{Remarks}
\def\uval{\overline{u} \left( t,x,\frac{\partial \overline{J}}{\partial x} \right)}
\begin{itemize}
\item Solving HJB \eqn{eq:hjb} is in general hard
    (analytically + computationally%
    \footnote{$\dim(x) \leq 10$})
\item Sometimes helpful:
    \begin{align}
    \txt{opt FB } &= \uval\\
    \ubar{t,x,\lambda} &= \argmin \set{
        f_0 \paren{\txu} + \lambda^Tf \paren{\txu}
    }
    \label{eq:hjb-umin-lambda}\\
    - \pdein{\Jbar{}}{t}
        &= f_0 \paren{t,x,\uval} \nonumber\\
        &\quad    + \underbrace{\pdein{\Jbar{t,x}}{x}}_{\lambda^T} f \paren{t,x,\uval}
            \label{eq:hjb-djdt}
    \end{align}
\end{itemize}

\paragraph{Example: LQR}
\begin{align*}
    \min    & \intdt{t_0}{t_f}{ x^T Q X + u^T R u}
                    + x_f^T S_f x_f,
                    \quad R >0, S_f > 0\\
    \st     & \quad \dot{x} = Ax + Bu
\end{align*}~

Find optimal feedback $\ubar{t,x}$
\begin{align*}
    \ubar{t,x} &= \argmin \set{ x^T Q X + u^T R u + \lambda^T(Ax + Bu) }
    \tag{\ref{eq:hjb-umin-lambda}}
\end{align*}
\begin{align*}
    \pde{u} \left( x^T Q X + \ubar{}^T R \ubar{} + \lambda^T(Ax + B\ubar{}) \right) &= 0^T\\
    2R\ubar{} + B^T\lambda &= 0\\
    \ubar{\lambda} & = -\frac{1}{2} R^{-1} B^T \lambda
\end{align*}
\begin{align*}
    - \pdein{\Jbar{}}{t}
        &= x^T Q x + \frac{1}{4} \lambda^T B \inv{R} B^T \lambda
            + \lambda^T A x\\
            &\quad + \lambda^T B ( -\frac{1}{2} R^{-1} B^T \lambda )
    \tag{\ref{eq:hjb-djdt}}\\
        &= x^T Q x - \frac{1}{4} \lambda^T B \inv{R} B^T \lambda
            + \lambda^T A x
            \numberthis \label{eq:lqr-djdt}\\
%        &= x^T Q x - \frac{1}{4} \pdein{\Jbar{}}{x} B \inv{R} B^T \left( \pde{\Jbar{}}{x} \right)^T
%            + \pdein{\Jbar{}}{x} A x
%            \numberthis \label{eq:lqr-djdt}
\end{align*}%
%
\begin{align*}
    \Jbar{t_f,x} &= x^T S_F x
    \tag{\ref{eq:hjb-final}}\\
    \txt{We try:} \quad \Jbar{t,x} &= x^T S(t) x, \txt{ with}\\
        \pdein{\Jbar{}}{t} &= x^T\dot{S}(t)x\\
        \pdein{\Jbar{}}{x} &= 2x^T S(t)= \lambda^T\\
        & \rightarrow \txt{ plug into } -\pdein{\Jbar{}}{t} \txt{ in } \eqn{eq:lqr-djdt}
\end{align*}
\begin{align*}
    -x^T \dot{S}(t) x
        &= x^T Q x - \frac{4}{4} x^T S(t) B \inv{R} B^T S(t) x\\
        &\quad + 2 x^T S(t) A x \quad \forall ~ x\\
    0   &= x^T \underbrace{ \paren{\dot{S}(t) + Q - S(t) B \inv{R} B^T S(t) + 2 S(t)A } }_{\overset{!}{=} 0} x
\end{align*}%
%
%
Ricatti equation (ODE)\footnote{PDE is converted into an ODE}:
\begin{align*}
    0 &= \dot{S}(t) + Q - S(t) B \inv{R} B^T S(t) + 2 S(t)A \numberthis
    \label{eq:ricatti}\\
    S(t_f) &= S_f \numberthis
\end{align*}%
%
\begin{align*}
    \ubar{\lambda} & = -\frac{1}{2} \inv{R} B^T \lambda
    = - \inv{R} B^T S(t) x
\end{align*}